.

theories/System/Lambda1.v
@@ -28,6 +28,7 @@ Class language : Type :=
   ; constants : Set
   ; signature (c : constants) : typ basic_types
   ; basic_types_hasEqDec :: hasEqDec@{Set} basic_types
+  ; constants_hasEqDec :: hasEqDec@{Set} constants
   }.
 
 End StlcLang.
@@ -75,6 +76,16 @@ Inductive trm : Set :=
   | App_trm (e1 : trm) (e2 : trm)
   | Lam_trm (y : name) (ty : typ) (e1 : trm)
   | Con_trm (c : L.(constants)).
+
+#[global]
+Instance trm_hasEqDec
+  : hasEqDec trm.
+Proof.
+  pose proof (name_hasEqDec) as HH1. do 1 red in HH1.
+  pose proof (typ_hasEqDec) as HH2. do 1 red in HH2.
+  pose proof (StlcLang.constants_hasEqDec) as HH3. do 1 red in HH3.
+  red. decide equality.
+Defined.
 
 Section FreeVariables.
 
@@ -724,7 +735,7 @@ Section AUX1.
 
 Fixpoint typ_height (ty : typ) : nat :=
   match ty with
-  | bty b => 0%nat
+  | bty b => 0
   | (ty1 -> ty2)%typ => 1 + max (typ_height ty1) (typ_height ty2)
   end.
 
@@ -745,11 +756,345 @@ Proof.
   - econs 4.
 Defined.
 
+Definition alpha_equiv (M : trm) (N : trm) : Prop :=
+  subst_trm nil_subst M = subst_trm nil_subst N.
+
+#[local] Infix "≡ₐ" := alpha_equiv.
+
+#[global]
+Instance alpha_equiv_Reflexive
+  : Reflexive alpha_equiv.
+Proof.
+  intros e. reflexivity.
+Qed.
+
+#[global]
+Instance alpha_equiv_Symmetric
+  : Symmetric alpha_equiv.
+Proof.
+  intros e1 e2 ALPHA. red in ALPHA |- *. symmetry. exact ALPHA.
+Qed.
+
+#[global]
+Instance alpha_equiv_Transitive
+  : Transitive alpha_equiv.
+Proof.
+  intros e1 e2 e3 ALPHA1 ALPHA2. red in ALPHA1, ALPHA2 |- *. congruence.
+Qed.
+
+#[global]
+Instance alpha_equiv_Equivalence
+  : Equivalence alpha_equiv.
+Proof.
+  split; [exact alpha_equiv_Reflexive | exact alpha_equiv_Symmetric | exact alpha_equiv_Transitive].
+Defined.
+
+Lemma alpha_equiv_subst_ext s1 s2 M
+  (EQUIV : forall z, is_free_in z M = true -> s1 z ≡ₐ s2 z)
+  : subst_trm s1 M ≡ₐ subst_trm s2 M.
+Proof.
+  red. do 2 rewrite <- subst_compose_spec.
+  eapply equiv_subst_implies_subst_same. intros z FREE.
+  unfold subst_compose. eapply EQUIV. exact FREE.
+Qed.
+
+Lemma alpha_equiv_subst_cons_compose x s N M
+  : subst_trm (cons_subst x (subst_trm s N) s) M ≡ₐ subst_trm s (subst_trm (one_subst x N) M).
+Proof.
+  transitivity (subst_trm (subst_compose (one_subst x N) s) M).
+  - eapply alpha_equiv_subst_ext. intros z FREE.
+    unfold subst_compose, one_subst, cons_subst.
+    destruct (eq_dec z x) as [EQ | NE].
+    + subst z. reflexivity.
+    + cbn. reflexivity.
+  - red. rewrite subst_compose_spec. reflexivity.
+Qed.
+
+Lemma alpha_equiv_one_subst z N N' M
+  (ALPHA : N ≡ₐ N')
+  : subst_trm (one_subst z N) M ≡ₐ subst_trm (one_subst z N') M.
+Proof.
+  red. repeat rewrite <- subst_compose_spec.
+  eapply equiv_subst_implies_subst_same. intros u FREE.
+  unfold subst_compose, one_subst, cons_subst, nil_subst.
+  destruct (eq_dec u z) as [EQ | NE].
+  - subst u. exact ALPHA.
+  - reflexivity.
+Qed.
+
+#[local] Opaque chi.
+
+Lemma alpha_equiv_beta_contract x x' ty M M' N N'
+  (ALPHA_LAM : Lam_trm x ty M ≡ₐ Lam_trm x' ty M')
+  (ALPHA_ARG : N ≡ₐ N')
+  : subst_trm (one_subst x N) M ≡ₐ subst_trm (one_subst x' N') M'.
+Proof.
+  red in ALPHA_LAM, ALPHA_ARG |- *. cbn -[chi] in ALPHA_LAM.
+  pose proof (subst_cons_lemma_aux1 N M nil_subst (chi nil_subst (Lam_trm x ty M)) x ty eq_refl) as EQ1.
+  pose proof (subst_cons_lemma_aux1 N' M' nil_subst (chi nil_subst (Lam_trm x' ty M')) x' ty eq_refl) as EQ2.
+  unfold one_subst. rewrite <- EQ1. rewrite <- EQ2.
+  assert (H_chi : chi nil_subst (Lam_trm x ty M) = chi nil_subst (Lam_trm x' ty M')).
+  { destruct (chi nil_subst (Lam_trm x ty M)) as [n1], (chi nil_subst (Lam_trm x' ty M')) as [n2]. now inversion ALPHA_LAM; subst. }
+  assert (H_body : subst_trm (cons_subst x (Var_trm (chi nil_subst (Lam_trm x ty M))) nil_subst) M = subst_trm (cons_subst x' (Var_trm (chi nil_subst (Lam_trm x' ty M'))) nil_subst) M').
+  { now inversion ALPHA_LAM. }
+  rewrite <- H_body. rewrite <- H_chi.
+  exact (alpha_equiv_one_subst _ _ _ _ ALPHA_ARG).
+Qed.
+
+Lemma subst_nil_precompose s M
+  : subst_trm (subst_compose s nil_subst) M = subst_trm (subst_compose s nil_subst) (subst_trm nil_subst M).
+Proof.
+  rewrite <- subst_compose_spec.
+  eapply equiv_subst_implies_subst_same. intros z FREE.
+  unfold subst_compose, nil_subst. reflexivity.
+Qed.
+
+Lemma alpha_equiv_subst_same s M M'
+  (ALPHA : M ≡ₐ M')
+  : subst_trm s M ≡ₐ subst_trm s M'.
+Proof.
+  red in ALPHA |- *.
+  do 2 rewrite <- subst_compose_spec.
+  rewrite subst_nil_precompose with (s := s) (M := M).
+  rewrite subst_nil_precompose with (s := s) (M := M').
+  now rewrite ALPHA.
+Qed.
+
+Lemma is_free_in_nil_subst z M
+  : is_free_in z (subst_trm nil_subst M) = true <-> is_free_in z M = true.
+Proof.
+  rewrite <- free_in_wrt_iff. unfold free_in_wrt, nil_subst.
+  split.
+  - intros [y [FREE FREE']]. cbn in FREE'.
+    apply eqb_spec in FREE'. subst y. exact FREE.
+  - intros FREE. exists z. split; [exact FREE | cbn].
+    rewrite eqb_spec. reflexivity.
+Qed.
+
+Lemma alpha_equiv_is_free_in z M M'
+  (ALPHA : M ≡ₐ M')
+  : is_free_in z M = is_free_in z M'.
+Proof.
+  destruct (is_free_in z M) eqn: FREE1, (is_free_in z M') eqn: FREE2; try reflexivity.
+  - exfalso.
+    pose proof (proj2 (is_free_in_nil_subst z M) FREE1) as FREE.
+    rewrite ALPHA in FREE.
+    rewrite is_free_in_nil_subst in FREE. congruence.
+  - exfalso.
+    pose proof (proj2 (is_free_in_nil_subst z M') FREE2) as FREE.
+    rewrite <- ALPHA in FREE.
+    rewrite is_free_in_nil_subst in FREE. congruence.
+Qed.
+
+Lemma alpha_equiv_chi_nil_lam x ty M M'
+  (ALPHA : M ≡ₐ M')
+  : chi nil_subst (Lam_trm x ty M) = chi nil_subst (Lam_trm x ty M').
+Proof.
+  eapply chi_frm_ext. intros z. unfold free_in_wrt, nil_subst.
+  assert (FREE_EQ : is_free_in z (Lam_trm x ty M) = is_free_in z (Lam_trm x ty M')).
+  { cbn. rewrite alpha_equiv_is_free_in with (z := z) (M := M) (M' := M'); eauto. }
+  split; intros [y [FREE FREE']]; cbn in FREE'; apply eqb_spec in FREE'; subst y; exists z; split; try (cbn; rewrite eqb_spec; reflexivity).
+  - now rewrite <- FREE_EQ.
+  - now rewrite FREE_EQ.
+Qed.
+
+Lemma subst_nil_renaming x z M
+  : subst_trm (cons_subst x (Var_trm z) nil_subst) M = subst_trm (cons_subst x (Var_trm z) nil_subst) (subst_trm nil_subst M).
+Proof.
+  set (s := cons_subst x (Var_trm z) nil_subst).
+  assert (EXT : forall u, subst_compose s nil_subst u = s u).
+  { intros u. unfold s, subst_compose, cons_subst, nil_subst. destruct (eq_dec u x); reflexivity. }
+  transitivity (subst_trm (subst_compose s nil_subst) M).
+  { symmetry. eapply equiv_subst_implies_subst_same. intros u FREE. exact (EXT u). }
+  rewrite subst_nil_precompose.
+  eapply equiv_subst_implies_subst_same.
+  intros u FREE. exact (EXT u).
+Qed.
+
+Lemma alpha_equiv_Lam_same x ty M M'
+  (ALPHA : M ≡ₐ M')
+  : Lam_trm x ty M ≡ₐ Lam_trm x ty M'.
+Proof.
+  red in ALPHA |- *. cbn -[chi].
+  pose proof (alpha_equiv_chi_nil_lam x ty M M' ALPHA) as H_chi.
+  rewrite H_chi. f_equal.
+  set (z := chi nil_subst (Lam_trm x ty M')).
+  rewrite subst_nil_renaming with (x := x) (z := z) (M := M).
+  rewrite ALPHA. symmetry. eapply subst_nil_renaming.
+Qed.
+
+#[global]
+Add Parametric Morphism
+  : Lam_trm with signature (eq ==> eq ==> alpha_equiv ==> alpha_equiv)
+  as Lam_alpha_alpha.
+Proof.
+  eapply alpha_equiv_Lam_same.
+Qed.
+
+Lemma alpha_equiv_nil_subst M
+  : M ≡ₐ subst_trm nil_subst M.
+Proof.
+  red. rewrite <- subst_compose_spec. eapply equiv_subst_implies_subst_same.
+  ii. reflexivity.
+Qed.
+
+Lemma alpha_equiv_App M M' N N'
+  (ALPHA1 : M ≡ₐ M')
+  (ALPHA2 : N ≡ₐ N')
+  : App_trm M N ≡ₐ App_trm M' N'.
+Proof.
+  red in ALPHA1, ALPHA2 |- *. simpl. congruence.
+Qed.
+
+#[global]
+Add Parametric Morphism
+  : App_trm with signature (alpha_equiv ==> alpha_equiv ==> alpha_equiv)
+  as App_alpha_alpha_alpha.
+Proof.
+  ii; eapply alpha_equiv_App; eauto.
+Qed.
+
+Lemma alpha_equiv_Var_inv x e
+  (ALPHA : Var_trm x ≡ₐ e)
+  : e = Var_trm x.
+Proof.
+  destruct e as [x' | M' N' | x' ty M' | c']; red in ALPHA; simpl in ALPHA; inv ALPHA.
+  reflexivity.
+Qed.
+
+Lemma alpha_equiv_App_inv M N e
+  (ALPHA : App_trm M N ≡ₐ e)
+  : exists M', exists N', e = App_trm M' N' /\ M ≡ₐ M' /\ N ≡ₐ N'.
+Proof.
+  destruct e as [x' | M' N' | x' ty' M' | c]; red in ALPHA; simpl in ALPHA; inv ALPHA.
+  exists M', N'. repeat split; try reflexivity; red; assumption.
+Qed.
+
+Lemma alpha_equiv_Lam_inv x ty M e
+  (ALPHA : Lam_trm x ty M ≡ₐ e)
+  : exists x', exists M', exists z, e = Lam_trm x' ty M' /\ subst_trm (one_subst x (Var_trm z)) M ≡ₐ subst_trm (one_subst x' (Var_trm z)) M'. 
+Proof.
+  destruct e as [x' | M' N' | x' ty' | c']; red in ALPHA; unfold nil_subst in ALPHA; simpl in ALPHA; try congruence.
+  assert (claim1 : ty = ty') by congruence.
+  subst ty'.
+  assert (claim2 : (chi (fun z : Name.t => Var_trm z) (Lam_trm x ty M)) = (chi (fun z : Name.t => Var_trm z) (Lam_trm x' ty e))) by congruence.
+  assert (claim3 : (subst_trm (cons_subst x (Var_trm (chi (fun z : Name.t => Var_trm z) (Lam_trm x ty M))) (fun z : Name.t => Var_trm z)) M) = (subst_trm (cons_subst x' (Var_trm (chi (fun z : Name.t => Var_trm z) (Lam_trm x' ty e))) (fun z : Name.t => Var_trm z)) e)) by congruence.
+  exists x'. exists e. exists (chi (fun z : Name.t => Var_trm z) (Lam_trm x' ty e)). split; eauto.
+  rewrite claim2 in claim3. unfold one_subst, nil_subst. rewrite claim3. reflexivity.
+Qed.
+
+Lemma alpha_equiv_Con_inv c e
+  (ALPHA : Con_trm c ≡ₐ e)
+  : e = Con_trm c.
+Proof.
+  destruct e as [x' | M' N' | x ty M' | c']; red in ALPHA; simpl in ALPHA; inv ALPHA.
+  reflexivity.
+Qed.
+
+Lemma alpha_equiv_dec M M'
+  : {M ≡ₐ M'} + {~ M ≡ₐ M'}.
+Proof.
+  unfold alpha_equiv. eapply trm_hasEqDec.
+Defined.
+
 Definition TypingSubst (Gamma : ctx) (gamma : subst) (Delta : ctx) : Set :=
   forall x, forall ty, Lookup x ty Delta -> Typing Gamma (gamma x) ty.
 
-Definition alpha_equiv (M : trm) (N : trm) : Prop :=
-  subst_trm nil_subst M = subst_trm nil_subst N.
+Lemma is_free_in_Lam_intro x y ty M
+  (NE : x <> y)
+  (FREE : is_free_in x M = true)
+  : is_free_in x (Lam_trm y ty M) = true.
+Proof.
+  simpl. unfold eqb. destruct (eq_dec x y) as [EQ | NE']; ss!.
+Qed.
+
+Lemma is_free_in_Var_refl x
+  : is_free_in x (Var_trm x) = true.
+Proof.
+  simpl. unfold eqb. destruct (eq_dec x x); ss!.
+Qed.
+
+Lemma Typing_context_invariance {Gamma : ctx} {Delta : ctx} {M : trm} {ty : typ}
+  (TYPING : Typing Gamma M ty)
+  (AGREE : forall x, forall ty, is_free_in x M = true -> Lookup x ty Gamma -> Lookup x ty Delta)
+  : Typing Delta M ty.
+Proof.
+  revert Delta AGREE. induction TYPING; simpl; intros Delta' AGREE.
+  - econs 1. eapply AGREE; [eapply is_free_in_Var_refl | exact LOOKUP].
+  - eapply App_typ with (ty1 := ty1).
+    + eapply IHTYPING1. intros x ty FREE LOOKUP.
+      eapply AGREE; [rewrite FREE; reflexivity | exact LOOKUP].
+    + eapply IHTYPING2. intros x ty FREE LOOKUP.
+      eapply AGREE; [rewrite FREE | exact LOOKUP].
+      destruct (is_free_in x e1); reflexivity.
+  - eapply Lam_typ with (ty2 := ty2). eapply IHTYPING. intros x ty FREE LOOKUP.
+    pattern LOOKUP. revert LOOKUP. eapply Lookup_cons.
+    + intros x_EQ ty_EQ. subst x ty.
+      exact (Lookup_Z y ty1 Delta' y ty1 eq_refl eq_refl).
+    + intros x_ne LOOKUP.
+      pose proof (COPY := x_ne). rewrite -> Name.ne_iff in COPY.
+      refine (Lookup_S x ty Delta' y ty1 x_ne (AGREE x ty (is_free_in_Lam_intro x y ty1 e1 COPY FREE) LOOKUP)).
+  - econs 4.
+Qed.
+
+Lemma Typing_shadowing {Gamma : ctx} {M : trm} {ty : typ} z z_ty
+  (TYPING : Typing Gamma M ty)
+  (NOT_FREE : is_free_in z M = false)
+  : Typing ((z, z_ty) :: Gamma) M ty.
+Proof.
+  eapply Typing_context_invariance; [exact TYPING |].
+  intros x ty' FREE LOOKUP.
+  destruct (eq_dec x z) as [EQ | NE].
+  - subst x. congruence.
+  - rewrite <- Name.ne_iff in NE.
+    exact (Lookup_S x ty' Gamma z z_ty NE LOOKUP).
+Qed.
+
+Lemma TypingSubst_preserves_Typing' Gamma gamma Delta M ty
+  (TYPING_SUBST : forall x, forall ty, is_free_in x M = true -> Lookup x ty Delta -> Typing Gamma (gamma x) ty)
+  (TYPING : Typing Delta M ty)
+  : Typing Gamma (subst_trm gamma M) ty.
+Proof.
+  revert Gamma gamma TYPING_SUBST.
+  induction TYPING; simpl; intros Gamma' gamma TYPING_SUBST.
+  - eapply TYPING_SUBST; [eapply is_free_in_Var_refl | exact LOOKUP].
+  - eapply App_typ with (ty1 := ty1).
+    + eapply IHTYPING1. intros x ty FREE LOOKUP.
+      eapply TYPING_SUBST; [rewrite FREE; reflexivity | exact LOOKUP].
+    + eapply IHTYPING2. intros x ty FREE LOOKUP.
+      eapply TYPING_SUBST; [rewrite FREE | exact LOOKUP].
+      destruct (is_free_in x e1); reflexivity.
+  - set (z := chi gamma (Lam_trm y ty1 e1)).
+    eapply Lam_typ with (ty2 := ty2). eapply IHTYPING. intros x ty FREE LOOKUP.
+    pattern LOOKUP. revert LOOKUP. eapply Lookup_cons.
+    + intros x_EQ ty_EQ. subst x ty.
+      unfold cons_subst. destruct (eq_dec y y) as [_ | CONTRA].
+      * econs 1. exact (Lookup_Z z ty1 Gamma' z ty1 eq_refl eq_refl).
+      * contradiction.
+    + intros x_ne LOOKUP.
+      unfold cons_subst. destruct (eq_dec x y) as [EQ | NE].
+      * subst x. pose proof (COPY := x_ne).
+        rewrite -> Name.ne_iff in COPY. contradiction.
+      * assert (LAM_FREE : is_free_in x (Lam_trm y ty1 e1) = true).
+        { eapply is_free_in_Lam_intro; eauto. }
+        eapply Typing_shadowing.
+        { eapply TYPING_SUBST; [exact LAM_FREE | exact LOOKUP]. }
+        pose proof (chi_is_fresh_in_subst (Lam_trm y ty1 e1) gamma) as FRESH.
+        unfold z. unfold is_fresh_in_subst in FRESH.
+        rewrite L.forallb_forall in FRESH. unfold "∘" in FRESH.
+        rewrite <- negb_true_iff. eapply FRESH.
+        rewrite <- is_free_in_iff. exact LAM_FREE.
+  - econs 4.
+Qed.
+
+Theorem TypingSubst_preserves_Typing Gamma gamma Delta M ty
+  (TYPING_SUBST : TypingSubst Gamma gamma Delta)
+  (TYPING : Typing Delta M ty)
+  : Typing Gamma (subst_trm gamma M) ty.
+Proof.
+  eapply TypingSubst_preserves_Typing'; [intros x ty' _ LOOKUP | exact TYPING].
+  eapply TYPING_SUBST. exact LOOKUP.
+Qed.
 
 End AUX1.
 
@@ -758,6 +1103,8 @@ Section BASIC_THEORY2_ON_SYNTAX.
 End BASIC_THEORY2_ON_SYNTAX.
 
 Section SN.
+
+#[local] Infix "≡ₐ" := alpha_equiv.
 
 Inductive fullBetaOnce : trm -> trm -> Prop :=
   | fullBetaOnce_beta x ty M N
@@ -771,74 +1118,118 @@ Inductive fullBetaOnce : trm -> trm -> Prop :=
   | fullBetaOnce_lam x ty M M'
     (BETA' : M ~>β M')
     : Lam_trm x ty M ~>β Lam_trm x ty M'
+  | fullBetaOnce_alpha M N N'
+    (BETA' : M ~>β N)
+    (ALPHA : N ≡ₐ N')
+    : M ~>β N'
   where "M ~>β N" := (fullBetaOnce M N).
 
-Inductive fullBetaMany (N : trm) : trm -> Prop :=
-  | fullBetaMany_init
-    : N ~>β* N
-  | fullBetaMany_step M M'
-    (STEP : M ~>β M')
-    (STEPS : M' ~>β* N)
+Inductive fullBetaMany (M : trm) (N : trm) : Set :=
+  | fullBetaMany_alpha
+    (ALPHA : M ≡ₐ N)
     : M ~>β* N
-  where "M ~>β* N" := (fullBetaMany N M).
+  | fullBetaMany_beta
+    (STEP : M ~>β N)
+    : M ~>β* N
+  | fullBetaMany_trans N'
+    (STEPS1 : M ~>β* N')
+    (STEPS2 : N' ~>β* N)
+    : M ~>β* N
+  where "M ~>β* N" := (fullBetaMany M N).
 
 #[local] Hint Constructors fullBetaMany : core.
 
+Lemma Var_stuck x
+  : forall N, ~ Var_trm x ~>β N.
+Proof.
+  intros N BETA.
+  remember (Var_trm x) as X eqn: EQ.
+  induction BETA; inv EQ; eauto.
+Qed.
+
+Lemma App_stuck M1 M2
+  (NOT_LAM : forall x, forall ty, forall M, ~ M1 = Lam_trm x ty M)
+  (NOT_BETA1 : forall N, ~ M1 ~>β N)
+  (NOT_BETA2 : forall N, ~ M2 ~>β N)
+  : forall N, ~ App_trm M1 M2 ~>β N.
+Proof.
+  intros N BETA.
+  remember (App_trm M1 M2) as X eqn: EQ.
+  induction BETA; inv EQ; eauto.
+  - contradiction (NOT_LAM x ty M eq_refl).
+  - eapply NOT_BETA1; eassumption.
+  - eapply NOT_BETA2; eassumption.
+Qed.
+
+Lemma Lam_stuck x ty M
+  (NOT_BETA : forall N, ~ M ~>β N)
+  : forall N, ~ Lam_trm x ty M ~>β N.
+Proof.
+  intros N BETA.
+  remember (Lam_trm x ty M) as X eqn: EQ.
+  induction BETA; inv EQ; eauto.
+  - eapply NOT_BETA; eassumption.
+Qed.
+
+Lemma Con_stuck c
+  : forall N, ~ Con_trm c~>β N.
+Proof.
+  intros N BETA.
+  remember (Con_trm c) as X eqn: EQ.
+  induction BETA; inv EQ; eauto.
+Qed.
+
 Lemma fullBetaOnce_dec (M : trm)
-  : B.sig trm (fun N => fullBetaOnce M N) + B.Prop_to_Set (forall N : trm, ~ fullBetaOnce M N).
+  : B.sig trm (fun N => M ~>β N) + B.Prop_to_Set (forall N : trm, ~ M ~>β N).
 Proof.
   induction M.
-  - right. red. intros N BETA. inv BETA.
+  - right. red. eapply Var_stuck.
   - destruct M1 as [x | M N | x ty M | c].
     + destruct IHM1 as [[N BETA1] | NOT_BETA1].
       { left. exists (App_trm N M2). econs 2. exact BETA1. }
       destruct IHM2 as [[N BETA2] | NOT_BETA2].
       { left. exists (App_trm (Var_trm x) N). econs 3. exact BETA2. }
-      right. red in NOT_BETA1, NOT_BETA2 |- *. intros N BETA. inv BETA.
-      { eapply NOT_BETA1. exact BETA'. }
-      { eapply NOT_BETA2. exact BETA'. }
+      right. red in NOT_BETA1, NOT_BETA2 |- *. eapply App_stuck; eauto; ii; congruence.
     + destruct IHM1 as [[N' BETA1] | NOT_BETA1].
       { left. exists (App_trm N' M2). econs 2. exact BETA1. }
       destruct IHM2 as [[N' BETA2] | NOT_BETA2].
       { left. exists (App_trm (App_trm M N) N'). econs 3. exact BETA2. }
-      right. red in NOT_BETA1, NOT_BETA2 |- *. intros N' BETA. inv BETA.
-      { eapply NOT_BETA1. exact BETA'. }
-      { eapply NOT_BETA2. exact BETA'. }
+      right. red in NOT_BETA1, NOT_BETA2 |- *. eapply App_stuck; eauto; ii; congruence.
     + left. exists (subst_trm (one_subst x M2) M). econs 1.
     + destruct IHM1 as [[N BETA1] | NOT_BETA1].
       { left. exists (App_trm N M2). econs 2. exact BETA1. }
       destruct IHM2 as [[N BETA2] | NOT_BETA2].
       { left. exists (App_trm (Con_trm c) N). econs 3. exact BETA2. }
-      right. red in NOT_BETA1, NOT_BETA2 |- *. intros N BETA. inv BETA.
-      { eapply NOT_BETA1. exact BETA'. }
-      { eapply NOT_BETA2. exact BETA'. }
+      right. red in NOT_BETA1, NOT_BETA2 |- *. eapply App_stuck; eauto; ii; congruence.
   - destruct IHM as [[N' BETA] | NOT_BETA1].
     + left. exists (Lam_trm y ty N'). econs 4. exact BETA.
-    + right. red in NOT_BETA1 |- *. intros N BETA. inv BETA.
-      eapply NOT_BETA1. exact BETA'.
-  - right. red. intros N BETA. inv BETA.
+    + right. red in NOT_BETA1 |- *. eapply Lam_stuck; eauto.
+  - right. red. eapply Con_stuck; eauto.
 Defined.
 
 Inductive sn (M : trm) : Prop :=
   | sn_intro
-    (sn_inv : forall N, fullBetaOnce M N -> sn N)
-    : sn M.
+    (sn_inv : forall N, M ~>β N -> sn N).
 
-Definition sn_inv {M : trm} (H_sn : sn M) : forall N, fullBetaOnce M N -> sn N :=
+Definition sn_inv {M : trm} (H_sn : sn M) : forall N, M ~>β N -> sn N :=
   match H_sn with
   | @sn_intro _ sn_inv => sn_inv
   end.
 
 Fixpoint normalize_with_sn (M : trm) (H_sn : sn M) {struct H_sn} : trm :=
   match fullBetaOnce_dec M with
-  | inl YES => let N : trm := B.proj1_sig YES in normalize_with_sn N (sn_inv H_sn N (B.proj2_sig YES))
+  | inl YES =>
+    let N : trm := B.proj1_sig YES in
+    normalize_with_sn N (sn_inv H_sn N (B.proj2_sig YES))
   | inr NO => M
   end.
 
 Lemma normalize_with_sn_unfold M H_sn :
   normalize_with_sn M H_sn =
   match fullBetaOnce_dec M with
-  | inl YES => let N : trm := B.proj1_sig YES in normalize_with_sn N (sn_inv H_sn N (B.proj2_sig YES))
+  | inl YES =>
+    let N : trm := B.proj1_sig YES in
+    normalize_with_sn N (sn_inv H_sn N (B.proj2_sig YES))
   | inr NO => M
   end.
 Proof.
@@ -852,7 +1243,7 @@ Proof.
   - reflexivity.
 Qed.
 
-Fixpoint normalize_with_sn_normalized (M : trm) (N : trm) (H_sn : sn M) {struct H_sn} : ~ fullBetaOnce (normalize_with_sn M H_sn) N.
+Fixpoint normalize_with_sn_normalized (M : trm) (N : trm) (H_sn : sn M) {struct H_sn} : ~ normalize_with_sn M H_sn ~>β N.
 Proof.
   destruct H_sn; simpl. intros BETA. destruct (fullBetaOnce_dec M) as [YES | NO].
   - eapply normalize_with_sn_normalized. exact BETA.
