theories/System/STLC.v
@@ -78,19 +78,20 @@ with typNf_betaNf Gamma v ty
   : (forall e, ~ fullBetaOnce v e).
 Proof.
   - destruct u_typNe; simpl.
-    + split; [eauto | intros e BETA]. inv BETA.
-    + split; [eauto | intros e BETA].
-      pose proof (typNe_betaNf Gamma u (ty -> ty')%typ u_typNe) as [claim1 claim2].
+    + split; [tauto | eapply Var_stuck].
+    + pose proof (typNe_betaNf Gamma u (ty -> ty')%typ u_typNe) as [claim1 claim2].
       pose proof (typNf_betaNf Gamma v ty v_typNf) as claim3.
-      clear typNe_betaNf typNf_betaNf. inv BETA; ss!.
-    + split; [eauto | intros e BETA]. inv BETA.
+      split; [tauto | eapply App_stuck].
+      * ii. subst u. contradiction claim1. red. tauto.
+      * exact claim2.
+      * exact claim3.
+    + split; [tauto | eapply Con_stuck].
   - destruct v_typNf; simpl.
     + intros e BETA.
       pose proof (typNe_betaNf Gamma u ty u_typNe) as [claim1 claim2].
       contradiction (claim2 e BETA).
-    + intros e BETA.
-      pose proof (typNf_betaNf ((x, ty) :: Gamma) v ty' v_typNf) as claim1.
-      clear typNe_betaNf typNf_betaNf. inv BETA; ss!.
+    + pose proof (typNf_betaNf ((x, ty) :: Gamma) v ty' v_typNf) as claim1.
+      eapply Lam_stuck. exact claim1.
 Qed.
 
 Lemma le_ctx_cons Gamma Delta x ty
@@ -539,6 +540,839 @@ Proof.
 Qed.
 
 End WEAK_NORMALISATION.
+
+Section STLC_SN.
+
+#[local] Opaque chi.
+
+#[local] Notation bty := (bty _).
+#[local] Infix "≡ₐ" := alpha_equiv : type_scope.
+#[local] Infix "~>β₁" := fullBetaOnce : type_scope.
+#[local] Infix "~>β*" := fullBetaMany : type_scope.
+#[local] Notation "Gamma ⊢ e ⦂ ty" := (Typing Gamma e ty).
+
+Inductive jmSN : trm L -> Prop :=
+  | jmSN_ne M
+    (NE : jmSNe M)
+    : jmSN M
+  | jmSN_lam x ty M
+    (BODY : jmSN M)
+    : jmSN (Lam_trm x ty M)
+  | jmSN_exp M N
+    (STEP : jmStep M N)
+    (N_SN : jmSN N)
+    : jmSN M
+with jmSNe : trm L -> Prop :=
+  | jmSNe_var x
+    : jmSNe (Var_trm x)
+  | jmSNe_con c
+    : jmSNe (Con_trm c)
+  | jmSNe_app M N
+    (M_NE : jmSNe M)
+    (N_SN : jmSN N)
+    : jmSNe (App_trm M N)
+with jmStep : trm L -> trm L -> Prop :=
+  | jmStep_beta x ty M N Q
+    (N_SN : jmSN N)
+    (ALPHA : subst_trm (one_subst x N) M ≡ₐ Q)
+    : jmStep (App_trm (Lam_trm x ty M) N) Q
+  | jmStep_appl M M' N
+    (STEP : jmStep M M')
+    : jmStep (App_trm M N) (App_trm M' N).
+
+Fixpoint jmRed (ty : typ L) : trm L -> Prop :=
+  match ty with
+  | bty b => jmSN
+  | (ty1 -> ty2)%typ => fun M => jmSN M /\ forall N, jmRed ty1 N -> jmRed ty2 (App_trm M N)
+  end.
+
+Fixpoint jmRed_jmSN (ty : typ L) {struct ty}
+  : forall M, jmRed ty M -> jmSN M.
+Proof.
+  destruct ty as [b | ty1 ty2]; simpl; intros M H.
+  - exact H.
+  - exact (proj1 H).
+Defined.
+
+Fixpoint jmRed_ne (ty : typ L)
+  : forall M, jmSNe M -> jmRed ty M.
+Proof.
+  destruct ty as [b | ty1 ty2]; simpl; intros M NE.
+  - eapply jmSN_ne. exact NE.
+  - split.
+    + eapply jmSN_ne. exact NE.
+    + intros N HN. eapply jmRed_ne.
+      eapply jmSNe_app.
+      * exact NE.
+      * eapply jmRed_jmSN. exact HN.
+Defined.
+
+Fixpoint jmRed_exp (ty : typ L) {struct ty}
+  : forall M, forall N, jmStep M N -> jmRed ty N -> jmRed ty M.
+Proof.
+  destruct ty as [b | ty1 ty2]; simpl; intros M N STEP HN.
+  - eapply jmSN_exp; eassumption.
+  - split.
+    + eapply jmSN_exp.
+      * exact STEP.
+      * exact (proj1 HN).
+    + intros P HP.
+      eapply jmRed_exp.
+      * eapply jmStep_appl. exact STEP.
+      * exact (proj2 HN P HP).
+Defined.
+
+Definition jmRedSubst (Gamma : ctx L) (gamma : subst L) : Prop :=
+  forall x, forall ty, Lookup x ty Gamma -> jmRed ty (gamma x).
+
+Lemma jmRedSubst_cons Gamma gamma x ty N
+  (N_RED : jmRed ty N)
+  (GAMMA_RED : jmRedSubst Gamma gamma)
+  : jmRedSubst ((x, ty) :: Gamma) (cons_subst x N gamma).
+Proof.
+  intros y ty'. unfold cons_subst. eapply Lookup_cons.
+  - intros y_eq ty_eq. subst y ty'. destruct (eq_dec x x) as [_ | NE].
+    + exact N_RED.
+    + contradiction.
+  - intros y_ne LOOKUP. destruct (eq_dec y x) as [EQ | NE].
+    + subst y. rewrite -> Name.ne_iff in y_ne. contradiction.
+    + eapply GAMMA_RED. exact LOOKUP.
+Defined.
+
+Lemma jmRedSubst_nil Gamma
+  : jmRedSubst Gamma nil_subst.
+Proof.
+  intros x ty LOOKUP. eapply jmRed_ne. eapply jmSNe_var.
+Defined.
+
+Theorem Typing_implies_jmRed Gamma e ty
+  (TYPING : Gamma ⊢ e ⦂ ty)
+  : forall gamma, jmRedSubst Gamma gamma -> jmRed ty (subst_trm gamma e).
+Proof.
+  induction TYPING; simpl; intros gamma GAMMA_RED.
+  - eapply GAMMA_RED. exact LOOKUP.
+  - eapply IHTYPING1.
+    { exact GAMMA_RED. }
+    eapply IHTYPING2. exact GAMMA_RED.
+  - set (z := chi gamma (Lam_trm y ty1 e1)).
+    split.
+    + eapply jmSN_lam. eapply jmRed_jmSN.
+      eapply IHTYPING. eapply jmRedSubst_cons.
+      * eapply jmRed_ne. eapply jmSNe_var.
+      * exact GAMMA_RED.
+    + intros N N_RED. eapply jmRed_exp.
+      * eapply jmStep_beta.
+        { eapply jmRed_jmSN. exact N_RED. }
+        { red. eapply subst_cons_lemma_aux1 with (ty := ty1). reflexivity. }
+      * eapply IHTYPING. eapply jmRedSubst_cons.
+        { exact N_RED. }
+        { exact GAMMA_RED. }
+  - eapply jmRed_ne. eapply jmSNe_con.
+Defined.
+
+Lemma alpha_equiv_lam_rename x ty M z
+  (NOT_FREE : is_free_in z (Lam_trm x ty M) = false)
+  : Lam_trm x ty M ≡ₐ
+    Lam_trm z ty (subst_trm (one_subst x (Var_trm z)) M).
+Proof.
+  red. simpl.
+  set (w := chi nil_subst (Lam_trm x ty M)).
+  enough (H_chi :
+    chi nil_subst (Lam_trm z ty (subst_trm (one_subst x (Var_trm z)) M)) = w).
+  { rewrite H_chi. unfold w. f_equal.
+    rewrite <- subst_compose_spec.
+    eapply equiv_subst_implies_subst_same. intros u FREE_u.
+    unfold subst_compose, one_subst, cons_subst, nil_subst.
+    destruct (eq_dec u x) as [u_eq_x | u_ne_x].
+    - subst u. simpl. destruct (eq_dec z z) as [_ | z_ne_z].
+      + reflexivity.
+      + contradiction.
+    - destruct (eq_dec u z) as [u_eq_z | u_ne_z].
+      + subst u. exfalso. simpl in NOT_FREE.
+        rewrite andb_false_iff in NOT_FREE. destruct NOT_FREE as [NOT_FREE | NOT_FREE].
+        * rewrite negb_false_iff in NOT_FREE. rewrite eqb_spec in NOT_FREE.
+          contradiction.
+        * rewrite <- not_true_iff_false in NOT_FREE. eapply NOT_FREE. exact FREE_u.
+      + simpl. destruct (eq_dec u z) as [u_eq_z | u_ne_z']; [contradiction | reflexivity].
+  }
+  subst w. eapply chi_frm_ext. intros u.
+  unfold free_in_wrt, nil_subst. split.
+  - intros (v & FREE_v & FREE_u). simpl in FREE_u.
+    rewrite eqb_spec in FREE_u. subst u. exists v. split; [| simpl; rewrite eqb_spec; reflexivity].
+    simpl in FREE_v. rewrite andb_true_iff in FREE_v.
+    destruct FREE_v as [v_ne_x FREE_v].
+    simpl. rewrite andb_true_iff. split.
+    + rewrite negb_true_iff. rewrite eqb_spec. intros v_eq_z.
+      subst v. rewrite <- free_in_wrt_iff in FREE_v.
+      destruct FREE_v as (u & FREE_u & FREE_v).
+      unfold one_subst, cons_subst, nil_subst in FREE_v.
+      destruct (eq_dec u x) as [u_eq_x | u_ne_x].
+      * subst u. simpl in FREE_v. rewrite eqb_spec in FREE_v.
+        rewrite negb_true_iff in v_ne_x. rewrite eqb_spec in v_ne_x.
+        contradiction.
+      * simpl in FREE_v. rewrite eqb_spec in FREE_v. subst u.
+        contradiction.
+    + rewrite <- free_in_wrt_iff in FREE_v.
+      destruct FREE_v as (u & FREE_u & FREE_v).
+      unfold one_subst, cons_subst, nil_subst in FREE_v.
+      destruct (eq_dec u x) as [u_eq_x | u_ne_x].
+      * subst u. simpl in FREE_v. rewrite eqb_spec in FREE_v. subst v.
+        rewrite negb_true_iff in v_ne_x. rewrite eqb_spec in v_ne_x.
+        contradiction.
+      * simpl in FREE_v. rewrite eqb_spec in FREE_v. subst v. exact FREE_u.
+  - intros (v & FREE_v & FREE_u). simpl in FREE_u.
+    rewrite eqb_spec in FREE_u. subst u.
+    simpl in FREE_v. rewrite andb_true_iff in FREE_v.
+    destruct FREE_v as [v_ne_z FREE_v].
+    exists v. split; [| simpl; rewrite eqb_spec; reflexivity].
+    simpl. rewrite andb_true_iff. split.
+    + rewrite negb_true_iff. rewrite eqb_spec. intros v_eq_z.
+      subst v. simpl in NOT_FREE. rewrite andb_false_iff in NOT_FREE.
+      destruct NOT_FREE as [NOT_FREE | NOT_FREE].
+      * rewrite negb_false_iff in NOT_FREE. rewrite eqb_spec in NOT_FREE.
+        rewrite negb_true_iff in v_ne_z. rewrite eqb_spec in v_ne_z.
+        contradiction.
+      * rewrite <- not_true_iff_false in NOT_FREE. eapply NOT_FREE.
+        exact FREE_v.
+    + rewrite <- free_in_wrt_iff. exists v. split.
+      * exact FREE_v.
+      * unfold one_subst, cons_subst, nil_subst.
+        destruct (eq_dec v x) as [v_eq_x | v_ne_x].
+        -- subst v. rewrite negb_true_iff in v_ne_z.
+           rewrite eqb_spec in v_ne_z. contradiction.
+        -- simpl. rewrite eqb_spec. reflexivity.
+Qed.
+
+Lemma fullBetaOnce_is_free_in M N z
+  (BETA : M ~>β₁ N)
+  (FREE : is_free_in z N = true)
+  : is_free_in z M = true.
+Proof.
+  induction BETA; simpl in *.
+  - rewrite <- free_in_wrt_iff in FREE.
+    destruct FREE as (y & FREE_M & FREE_s).
+    unfold one_subst, cons_subst, nil_subst in FREE_s.
+    destruct (eq_dec y x) as [y_eq_x | y_ne_x].
+    + subst y. rewrite orb_true_iff. right. exact FREE_s.
+    + simpl in FREE_s. rewrite eqb_spec in FREE_s. subst z.
+      rewrite orb_true_iff. left. rewrite andb_true_iff. split.
+      * rewrite negb_true_iff. rewrite eqb_spec. intros z_eq_x.
+        contradiction y_ne_x.
+      * exact FREE_M.
+  - rewrite orb_true_iff in FREE |- *. destruct FREE as [FREE | FREE].
+    + left. eapply IHBETA. exact FREE.
+    + right. exact FREE.
+  - rewrite orb_true_iff in FREE |- *. destruct FREE as [FREE | FREE].
+    + left. exact FREE.
+    + right. eapply IHBETA. exact FREE.
+  - rewrite andb_true_iff in FREE |- *. destruct FREE as [FREE1 FREE2].
+    split.
+    + exact FREE1.
+    + eapply IHBETA. exact FREE2.
+  - eapply IHBETA.
+    rewrite alpha_equiv_is_free_in with (M := N) (M' := N'); eassumption.
+Qed.
+
+Lemma fullBetaOnce_preserves_is_fresh_in_subst s M N z
+  (BETA : M ~>β₁ N)
+  (FRESH : is_fresh_in_subst z s M = true)
+  : is_fresh_in_subst z s N = true.
+Proof.
+  unfold is_fresh_in_subst in *. rewrite forallb_forall in FRESH |- *.
+  intros x x_in. eapply FRESH.
+  rewrite <- is_free_in_iff in x_in. rewrite <- is_free_in_iff.
+  eapply fullBetaOnce_is_free_in; eassumption.
+Qed.
+
+Lemma alpha_equiv_subst_lam_fresh s x ty M z
+  (FRESH : is_fresh_in_subst z s (Lam_trm x ty M) = true)
+  : subst_trm s (Lam_trm x ty M) ≡ₐ Lam_trm z ty (subst_trm (cons_subst x (Var_trm z) s) M).
+Proof.
+  simpl. set (w := chi s (Lam_trm x ty M)).
+  transitivity (Lam_trm z ty (subst_trm (one_subst w (Var_trm z)) (subst_trm (cons_subst x (Var_trm w) s) M))).
+  - eapply alpha_equiv_lam_rename.
+    change (is_free_in z (subst_trm s (Lam_trm x ty M)) = false).
+    rewrite <- is_fresh_in_subst_iff. exact FRESH.
+  - eapply alpha_equiv_Lam_same. red.
+    unfold w. eapply subst_cons_lemma_aux1 with (ty := ty). reflexivity.
+Qed.
+
+#[local] Reserved Infix "~>β₀" (at level 70).
+
+#[local] Reserved Infix "~>β₀*" (at level 70).
+
+Inductive rawBetaOnce : trm L -> trm L -> Prop :=
+  | rawBetaOnce_beta x ty M N
+    : (App_trm (Lam_trm x ty M) N) ~>β₀ (subst_trm (one_subst x N) M)
+  | rawBetaOnce_appl M M' N
+    (BETA : M ~>β₀ M')
+    : (App_trm M N) ~>β₀ (App_trm M' N)
+  | rawBetaOnce_appr M N N'
+    (BETA : N ~>β₀ N')
+    : (App_trm M N) ~>β₀ (App_trm M N')
+  | rawBetaOnce_lam x ty M M'
+    (BETA : M ~>β₀ M')
+    : (Lam_trm x ty M) ~>β₀ (Lam_trm x ty M')
+  where "M ~>β₀ N" := (rawBetaOnce M N).
+
+Inductive rawBetaMany (M : trm L) (N : trm L) : Prop :=
+  | rawBetaMany_alpha
+    (ALPHA : M ≡ₐ N)
+    : M ~>β₀* N
+  | rawBetaMany_beta
+    (STEP : M ~>β₀ N)
+    : M ~>β₀* N
+  | rawBetaMany_trans M'
+    (STEPS1 : M ~>β₀* M')
+    (STEPS2 : M' ~>β₀* N)
+    : M ~>β₀* N
+  where "M ~>β₀* N" := (rawBetaMany M N).
+
+Inductive raw_sn (M : trm L) : Prop :=
+  | raw_sn_intro
+    (raw_sn_inv : forall N, M ~>β₀ N -> raw_sn N).
+
+Definition raw_sn_inv {M : trm L} (H_sn : raw_sn M) : forall N, M ~>β₀ N -> raw_sn N :=
+  match H_sn with
+  | @raw_sn_intro _ raw_sn_inv => raw_sn_inv
+  end.
+
+Lemma rawBetaOnce_fullBetaOnce M N
+  (BETA : M ~>β₀ N)
+  : M ~>β₁ N.
+Proof.
+  induction BETA; eauto using fullBetaOnce.
+Qed.
+
+Lemma fullBetaOnce_rawBetaOnce M N
+  (BETA : M ~>β₁ N)
+  : exists P, M ~>β₀ P /\ P ≡ₐ N.
+Proof.
+  induction BETA.
+  - exists (subst_trm (one_subst x N) M). split; [econs 1 | reflexivity].
+  - destruct IHBETA as (P & STEP & ALPHA).
+    exists (App_trm P N). split; [econs 2; exact STEP | ].
+    eapply alpha_equiv_App; [exact ALPHA | reflexivity].
+  - destruct IHBETA as (P & STEP & ALPHA).
+    exists (App_trm M P). split; [econs 3; exact STEP | ].
+    eapply alpha_equiv_App; [reflexivity | exact ALPHA].
+  - destruct IHBETA as (P & STEP & ALPHA).
+    exists (Lam_trm x ty P). split; [econs 4; exact STEP | ].
+    eapply alpha_equiv_Lam_same. exact ALPHA.
+  - destruct IHBETA as (P & STEP & ALPHA').
+    exists P. split; [exact STEP | ].
+    transitivity N; eassumption.
+Qed.
+
+Lemma rawBetaOnce_preserves_is_fresh_in_subst s M N z
+  (BETA : M ~>β₀ N)
+  (FRESH : is_fresh_in_subst z s M = true)
+  : is_fresh_in_subst z s N = true.
+Proof.
+  eapply fullBetaOnce_preserves_is_fresh_in_subst.
+  - eapply rawBetaOnce_fullBetaOnce. exact BETA.
+  - exact FRESH.
+Qed.
+
+Lemma rawBetaOnce_subst_compat s M N
+  (BETA : M ~>β₀ N)
+  : exists P, subst_trm s M ~>β₀ P /\ P ≡ₐ subst_trm s N.
+Proof.
+  revert s. induction BETA; intros s; simpl.
+  - set (z := chi s (Lam_trm x ty M)).
+    exists (subst_trm (one_subst z (subst_trm s N)) (subst_trm (cons_subst x (Var_trm z) s) M)).
+    split.
+    + econs 1.
+    + transitivity (subst_trm (cons_subst x (subst_trm s N) s) M).
+      * red. unfold z. eapply subst_cons_lemma_aux1 with (ty := ty).
+        reflexivity.
+      * eapply alpha_equiv_subst_cons_compose.
+  - pose proof (IHBETA s) as (P & STEP & ALPHA).
+    exists (App_trm P (subst_trm s N)). split.
+    + econs 2. exact STEP.
+    + eapply alpha_equiv_App; [exact ALPHA | reflexivity].
+  - pose proof (IHBETA s) as (P & STEP & ALPHA).
+    exists (App_trm (subst_trm s M) P). split.
+    + econs 3. exact STEP.
+    + eapply alpha_equiv_App; [reflexivity | exact ALPHA].
+  - set (z := chi s (Lam_trm x ty M)).
+    destruct IHBETA with (s := cons_subst x (Var_trm z) s) as (P & STEP & ALPHA).
+    exists (Lam_trm z ty P). split.
+    + econs 4. exact STEP.
+    + transitivity (Lam_trm z ty (subst_trm (cons_subst x (Var_trm z) s) M')).
+      * eapply alpha_equiv_Lam_same. exact ALPHA.
+      * symmetry. eapply alpha_equiv_subst_lam_fresh.
+        unfold z. eapply rawBetaOnce_preserves_is_fresh_in_subst.
+        { econs 4. exact BETA. }
+        { eapply chi_is_fresh_in_subst. }
+Qed.
+
+Lemma alpha_equiv_one_subst_self x M
+  : subst_trm (one_subst x (Var_trm x)) M ≡ₐ M.
+Proof.
+  transitivity (subst_trm nil_subst M).
+  - eapply alpha_equiv_subst_ext. intros z FREE.
+    unfold one_subst, cons_subst, nil_subst.
+    destruct (eq_dec z x) as [z_eq_x | z_ne_x]; subst; reflexivity.
+  - symmetry. eapply alpha_equiv_nil_subst.
+Qed.
+
+Lemma alpha_equiv_Lam_inv_body_left x y ty M N
+  (ALPHA : Lam_trm x ty M ≡ₐ Lam_trm y ty N)
+  : M ≡ₐ subst_trm (one_subst y (Var_trm x)) N.
+Proof.
+  transitivity (subst_trm (one_subst x (Var_trm x)) M).
+  - symmetry. eapply alpha_equiv_one_subst_self.
+  - eapply alpha_equiv_beta_contract.
+    + exact ALPHA.
+    + reflexivity.
+Qed.
+
+Lemma alpha_rawBetaOnce_comm M
+  : forall N, forall P, M ≡ₐ N -> N ~>β₀ P -> exists Q, M ~>β₀ Q /\ Q ≡ₐ P.
+Proof.
+  induction M as [x | M1 IH1 M2 IH2 | x ty M IH | c]; intros N P ALPHA BETA.
+  - pose proof (alpha_equiv_Var_inv x N ALPHA) as N_eq.
+    subst N. inversion BETA.
+  - pose proof (alpha_equiv_App_inv M1 M2 N ALPHA) as (N1 & N2 & N_eq & ALPHA1 & ALPHA2).
+    subst N. inversion BETA; subst.
+    + assert (ALPHA1' : Lam_trm x ty M ≡ₐ M1) by (symmetry; exact ALPHA1).
+      pose proof (alpha_equiv_Lam_inv x ty M M1 ALPHA1') as (x' & M' & z & M1_eq & BODY_ALPHA).
+      subst M1. exists (subst_trm (one_subst x' M2) M'). split.
+      * econs 1.
+      * assert (ALPHA_ARG : N2 ≡ₐ M2) by (symmetry; exact ALPHA2).
+        symmetry. exact (alpha_equiv_beta_contract x x' ty M M' N2 M2 ALPHA1' ALPHA_ARG).
+    + pose proof (IH1 N1 M' ALPHA1 BETA0) as (Q & STEP & ALPHA_Q).
+      exists (App_trm Q M2). split.
+      * econs 2. exact STEP.
+      * eapply alpha_equiv_App; [exact ALPHA_Q | exact ALPHA2].
+    + pose proof (IH2 N2 N' ALPHA2 BETA0) as (Q & STEP & ALPHA_Q).
+      exists (App_trm M1 Q). split.
+      * econs 3. exact STEP.
+      * eapply alpha_equiv_App; [exact ALPHA1 | exact ALPHA_Q].
+  - pose proof (alpha_equiv_Lam_inv x ty M N ALPHA) as (y & N' & z & N_eq & BODY_ALPHA).
+    subst N. inversion BETA; subst.
+    pose proof (rawBetaOnce_subst_compat (one_subst y (Var_trm x)) _ _ BETA0) as (R & STEP & ALPHA_R).
+    pose proof (alpha_equiv_Lam_inv_body_left x y ty M N' ALPHA) as BODY_ALPHA'.
+    pose proof (IH _ _ BODY_ALPHA' STEP) as (Q & STEP_Q & ALPHA_Q).
+    exists (Lam_trm x ty Q). split.
+    + econs 4. exact STEP_Q.
+    + transitivity (Lam_trm x ty R).
+      { eapply alpha_equiv_Lam_same. exact ALPHA_Q. }
+      transitivity (Lam_trm x ty (subst_trm (one_subst y (Var_trm x)) M')).
+      { eapply alpha_equiv_Lam_same. exact ALPHA_R. }
+      { symmetry. eapply alpha_equiv_lam_rename.
+        assert (NOT_FREE_SOURCE : is_free_in x (Lam_trm x ty M) = false).
+        { simpl. unfold eqb. destruct (eq_dec x x) as [_ | NE].
+          - reflexivity.
+          - contradiction.
+        }
+        assert (NOT_FREE_N : is_free_in x (Lam_trm y ty N') = false).
+        { rewrite <- alpha_equiv_is_free_in with (M := Lam_trm x ty M) (M' := Lam_trm y ty N'); eassumption. }
+        destruct (is_free_in x (Lam_trm y ty M')) eqn:FREE; [| reflexivity].
+        pose proof (fullBetaOnce_is_free_in _ _ x (rawBetaOnce_fullBetaOnce _ _ (rawBetaOnce_lam y ty N' M' BETA0)) FREE) as FREE_N.
+        congruence.
+      }
+  - pose proof (alpha_equiv_Con_inv c N ALPHA) as N_eq.
+    subst N. inversion BETA.
+Qed.
+
+Fixpoint raw_sn_alpha (M : trm L) (M_SN : raw_sn M) {struct M_SN} : forall N, M ≡ₐ N -> raw_sn N.
+Proof.
+  destruct M_SN as [M_SN]. intros N ALPHA. econs. intros P BETA.
+  pose proof (alpha_rawBetaOnce_comm M N P ALPHA BETA) as (Q & STEP & ALPHA_Q).
+  eapply raw_sn_alpha.
+  - eapply M_SN. exact STEP.
+  - exact ALPHA_Q.
+Defined.
+
+Lemma rawBetaMany_preserves_raw_sn M N
+  (STEPS : M ~>β₀* N)
+  (M_SN : raw_sn M)
+  : raw_sn N.
+Proof.
+  induction STEPS.
+  - eapply raw_sn_alpha; eassumption.
+  - eapply raw_sn_inv; eassumption.
+  - eapply IHSTEPS2. eapply IHSTEPS1. exact M_SN.
+Qed.
+
+Lemma rawBetaMany_app_l M M' N
+  (STEPS : M ~>β₀* M')
+  : App_trm M N ~>β₀* App_trm M' N.
+Proof.
+  induction STEPS.
+  - econs 1. eapply alpha_equiv_App; [exact ALPHA | reflexivity].
+  - econs 2. econs 2. exact STEP.
+  - econs 3; eassumption.
+Qed.
+
+Lemma rawBetaMany_app_r M N N'
+  (STEPS : N ~>β₀* N')
+  : App_trm M N ~>β₀* App_trm M N'.
+Proof.
+  induction STEPS.
+  - econs 1. eapply alpha_equiv_App; [reflexivity | exact ALPHA].
+  - econs 2. econs 3. exact STEP.
+  - econs 3; eassumption.
+Qed.
+
+Lemma rawBetaMany_lam x ty M M'
+  (STEPS : M ~>β₀* M')
+  : Lam_trm x ty M ~>β₀* Lam_trm x ty M'.
+Proof.
+  induction STEPS.
+  - econs 1. eapply alpha_equiv_Lam_same. exact ALPHA.
+  - econs 2. econs 4. exact STEP.
+  - econs 3; eassumption.
+Qed.
+
+Lemma alpha_equiv_subst_shadow x A gamma M
+  : subst_trm (cons_subst x A (cons_subst x A gamma)) M ≡ₐ
+    subst_trm (cons_subst x A gamma) M.
+Proof.
+  eapply alpha_equiv_subst_ext. intros z FREE.
+  unfold cons_subst. destruct (eq_dec z x); reflexivity.
+Qed.
+
+Lemma alpha_equiv_subst_swap x y A B gamma M
+  (NE : y <> x)
+  : subst_trm (cons_subst y B (cons_subst x A gamma)) M ≡ₐ
+    subst_trm (cons_subst x A (cons_subst y B gamma)) M.
+Proof.
+  eapply alpha_equiv_subst_ext. intros z FREE.
+  unfold cons_subst.
+  destruct (eq_dec z y) as [z_eq_y | z_ne_y].
+  - subst z. destruct (eq_dec y x) as [y_eq_x | y_ne_x].
+    + contradiction.
+    + reflexivity.
+  - destruct (eq_dec z x) as [z_eq_x | z_ne_x].
+    + reflexivity.
+    + destruct (eq_dec z y) as [z_eq_y | z_ne_y']; [contradiction | reflexivity].
+Qed.
+
+Lemma rawBetaOnce_preserves_is_fresh_in_subst_update gamma x N N' z M
+  (BETA : N ~>β₀ N')
+  (FRESH : is_fresh_in_subst z (cons_subst x N gamma) M = true)
+  : is_fresh_in_subst z (cons_subst x N' gamma) M = true.
+Proof.
+  unfold is_fresh_in_subst in *. rewrite forallb_forall in FRESH |- *.
+  intros y y_in. specialize (FRESH y y_in).
+  unfold "∘" in FRESH |- *. unfold cons_subst in FRESH |- *.
+  destruct (eq_dec y x) as [y_eq_x | y_ne_x].
+  - rewrite negb_true_iff in FRESH |- *.
+    destruct (is_free_in z N') eqn:FREE; [| reflexivity].
+    pose proof (fullBetaOnce_is_free_in _ _ z (rawBetaOnce_fullBetaOnce _ _ BETA) FREE) as FREE_N.
+    congruence.
+  - exact FRESH.
+Qed.
+
+Lemma rawBetaMany_subst_update gamma x N N' M
+  (BETA : N ~>β₀ N')
+  : subst_trm (cons_subst x N gamma) M ~>β₀*
+    subst_trm (cons_subst x N' gamma) M.
+Proof.
+  revert gamma x N N' BETA. induction M; intros gamma x0 N N' BETA; simpl.
+  - unfold cons_subst. destruct (eq_dec x x0) as [x_eq | x_ne].
+    + subst x. econs 2. exact BETA.
+    + econs 1. reflexivity.
+  - eapply rawBetaMany_trans with (M' := App_trm (subst_trm (cons_subst x0 N' gamma) M1) (subst_trm (cons_subst x0 N gamma) M2)).
+    + eapply rawBetaMany_app_l. eapply IHM1. exact BETA.
+    + eapply rawBetaMany_app_r. eapply IHM2. exact BETA.
+  - set (s := cons_subst x0 N gamma).
+    set (s' := cons_subst x0 N' gamma).
+    set (z := chi s (Lam_trm y ty M)).
+    eapply rawBetaMany_trans with (M' := Lam_trm z ty (subst_trm (cons_subst y (Var_trm z) s') M)).
+    + eapply rawBetaMany_lam.
+      destruct (eq_dec y x0) as [y_eq_x | y_ne_x].
+      * subst y. econs 1.
+        unfold s, s'. eapply alpha_equiv_subst_ext. intros u FREE.
+        unfold cons_subst. destruct (eq_dec u x0); reflexivity.
+      * eapply rawBetaMany_trans with (M' := subst_trm (cons_subst x0 N (cons_subst y (Var_trm z) gamma)) M).
+        { econs 1. unfold s. eapply alpha_equiv_subst_swap. exact y_ne_x. }
+        eapply rawBetaMany_trans with (M' := subst_trm (cons_subst x0 N' (cons_subst y (Var_trm z) gamma)) M).
+        { eapply IHM. exact BETA. }
+        { econs 1. symmetry. unfold s'. eapply alpha_equiv_subst_swap. exact y_ne_x. }
+    + econs 1. symmetry. eapply alpha_equiv_subst_lam_fresh.
+      unfold z, s, s'. eapply rawBetaOnce_preserves_is_fresh_in_subst_update.
+      * exact BETA.
+      * eapply chi_is_fresh_in_subst.
+  - econs 1. reflexivity.
+Qed.
+
+Lemma rawBetaMany_one_subst_arg x M N N'
+  (BETA : N ~>β₀ N')
+  : subst_trm (one_subst x N) M ~>β₀* subst_trm (one_subst x N') M.
+Proof.
+  unfold one_subst. eapply rawBetaMany_subst_update. exact BETA.
+Qed.
+
+Inductive neutral : trm L -> Prop :=
+  | neutral_var x
+    : neutral (Var_trm x)
+  | neutral_con c
+    : neutral (Con_trm c)
+  | neutral_app M N
+    (NE : neutral M)
+    : neutral (App_trm M N).
+
+Lemma neutral_not_lam M x ty N
+  (NE : neutral M)
+  (EQ : M = Lam_trm x ty N)
+  : False.
+Proof.
+  revert EQ; induction NE; intros EQ; inv EQ.
+Qed.
+
+Lemma neutral_rawBetaOnce M N
+  (NE : neutral M)
+  (BETA : M ~>β₀ N)
+  : neutral N.
+Proof.
+  revert N BETA. induction NE; intros P BETA; inversion BETA; subst; eauto using neutral.
+  contradiction (neutral_not_lam _ _ _ _ NE eq_refl).
+Qed.
+
+Lemma raw_sn_var x
+  : raw_sn (Var_trm x).
+Proof.
+  econs. intros N BETA. inversion BETA.
+Qed.
+
+Lemma raw_sn_con c
+  : raw_sn (Con_trm c).
+Proof.
+  econs. intros N BETA. inversion BETA.
+Qed.
+
+Fixpoint raw_sn_lam (M : trm L) (M_SN : raw_sn M) {struct M_SN} : forall x, forall ty, raw_sn (Lam_trm x ty M).
+Proof.
+  destruct M_SN as [M_SN]. econs. intros N BETA.
+  inversion BETA; subst. eapply raw_sn_lam. eapply M_SN. exact BETA0.
+Defined.
+
+Lemma raw_sn_app_neutral M N
+  (NE : neutral M)
+  (M_SN : raw_sn M)
+  (N_SN : raw_sn N)
+  : raw_sn (App_trm M N).
+Proof.
+  revert N NE N_SN. induction M_SN as [M M_SN IHM]; intros N NE N_SN.
+  induction N_SN as [N N_SN IHN]. econs. intros P BETA.
+  inversion BETA; subst.
+  - contradiction (neutral_not_lam _ _ _ _ NE eq_refl).
+  - eapply IHM.
+    + exact BETA0.
+    + eapply neutral_rawBetaOnce; eassumption.
+    + econs. exact N_SN.
+  - eapply IHN. exact BETA0.
+Qed.
+
+Lemma raw_wkh_exp_alpha x ty M N Q
+  (N_SN : raw_sn N)
+  (Q_SN : raw_sn Q)
+  (ALPHA : Q ≡ₐ subst_trm (one_subst x N) M)
+  : raw_sn (App_trm (Lam_trm x ty M) N).
+Proof.
+  revert M Q Q_SN ALPHA. induction N_SN as [N N_SN IHN].
+  intros M Q Q_SN ALPHA.
+  revert M ALPHA. induction Q_SN as [Q Q_SN IHQ].
+  intros M ALPHA. econs. intros P BETA. inversion BETA; subst.
+  - eapply raw_sn_alpha.
+    + econs. exact Q_SN.
+    + exact ALPHA.
+  - inversion BETA0; subst.
+    pose proof (rawBetaOnce_subst_compat (one_subst x N) _ _ BETA1) as (R & STEP_R & ALPHA_R).
+    pose proof (alpha_rawBetaOnce_comm Q (subst_trm (one_subst x N) M) R ALPHA STEP_R) as (S & STEP_S & ALPHA_S).
+    eapply IHQ.
+    + exact STEP_S.
+    + transitivity R; [exact ALPHA_S | exact ALPHA_R].
+  - eapply IHN.
+    + exact BETA0.
+    + eapply rawBetaMany_preserves_raw_sn.
+      * eapply rawBetaMany_one_subst_arg. exact BETA0.
+      * eapply raw_sn_alpha.
+        { econs. exact Q_SN. }
+        { exact ALPHA. }
+    + reflexivity.
+Qed.
+
+Lemma raw_wkh_exp x ty M N
+  (N_SN : raw_sn N)
+  (BODY_SN : raw_sn (subst_trm (one_subst x N) M))
+  : raw_sn (App_trm (Lam_trm x ty M) N).
+Proof.
+  eapply raw_wkh_exp_alpha; [exact N_SN | exact BODY_SN | reflexivity].
+Qed.
+
+Inductive rawHeadStep : trm L -> trm L -> Prop :=
+  | rawHeadStep_beta x ty M N Q
+    (N_SN : raw_sn N)
+    (ALPHA : Q ≡ₐ subst_trm (one_subst x N) M)
+    : rawHeadStep (App_trm (Lam_trm x ty M) N) Q
+  | rawHeadStep_appl M M' N
+    (STEP : rawHeadStep M M')
+    : rawHeadStep (App_trm M N) (App_trm M' N).
+
+Lemma rawHeadStep_not_lam M N x ty P
+  (STEP : rawHeadStep M N)
+  (EQ : M = Lam_trm x ty P)
+  : False.
+Proof.
+  revert EQ; induction STEP; intros EQ; inv EQ.
+Qed.
+
+Lemma rawHead_confluence M N P
+  (STEP : rawHeadStep M N)
+  (BETA : M ~>β₀ P)
+  : N ≡ₐ P \/ (exists Q, rawHeadStep P Q /\ N ~>β₀* Q).
+Proof.
+  revert P BETA. induction STEP; intros P BETA; inversion BETA; subst.
+  - left. exact ALPHA.
+  - inversion BETA0; subst.
+    pose proof (rawBetaOnce_subst_compat (one_subst x N) _ _ BETA1) as (R & STEP_R & ALPHA_R).
+    right. exists (subst_trm (one_subst x N) M'0). split.
+    + econs 1; [exact N_SN | reflexivity].
+    + eapply rawBetaMany_trans with (M' := subst_trm (one_subst x N) M).
+      * econs 1. exact ALPHA.
+      * eapply rawBetaMany_trans with (M' := R).
+        { econs 2. exact STEP_R. }
+        { econs 1. exact ALPHA_R. }
+  - right. exists (subst_trm (one_subst x N') M). split.
+    + econs 1.
+      * eapply raw_sn_inv; eassumption.
+      * reflexivity.
+    + eapply rawBetaMany_trans with (M' := subst_trm (one_subst x N) M).
+      * econs 1. exact ALPHA.
+      * eapply rawBetaMany_one_subst_arg. exact BETA0.
+  - contradiction (rawHeadStep_not_lam _ _ _ _ _ STEP eq_refl).
+  - pose proof (IHSTEP M'0 BETA0) as [ALPHA_STEP | (Q & STEP_Q & MANY_Q)].
+    + left. eapply alpha_equiv_App; [exact ALPHA_STEP | reflexivity].
+    + right. exists (App_trm Q N). split.
+      * econs 2. exact STEP_Q.
+      * eapply rawBetaMany_app_l. exact MANY_Q.
+  - right. exists (App_trm M' N'). split.
+    + econs 2. exact STEP.
+    + eapply rawBetaMany_app_r. econs 2. exact BETA0.
+Qed.
+
+Fixpoint raw_sn_app_inv M N
+  (MN_SN : raw_sn (App_trm M N)) {struct MN_SN}
+  : raw_sn M /\ raw_sn N.
+Proof.
+  destruct MN_SN as [MN_SN]. split.
+  - econs. intros M' BETA.
+    exact (proj1 (raw_sn_app_inv M' N (MN_SN (App_trm M' N) (rawBetaOnce_appl M M' N BETA)))).
+  - econs. intros N' BETA.
+    exact (proj2 (raw_sn_app_inv M N' (MN_SN (App_trm M N') (rawBetaOnce_appr M N N' BETA)))).
+Defined.
+
+Lemma rawHead_backward_aux M N M'
+  (M_SN : raw_sn M)
+  (N_SN : raw_sn N)
+  (STEP : rawHeadStep M M')
+  (M'N_SN : raw_sn (App_trm M' N))
+  : raw_sn (App_trm M N).
+Proof.
+  revert N M' N_SN STEP M'N_SN.
+  induction M_SN as [M M_SN IHM]; intros N M' N_SN STEP M'N_SN.
+  revert M' STEP M'N_SN.
+  induction N_SN as [N N_SN IHN]; intros M' STEP M'N_SN.
+  econs. intros Q BETA. inversion BETA; subst.
+  - contradiction (rawHeadStep_not_lam _ _ _ _ _ STEP eq_refl).
+  - pose proof (rawHead_confluence M M' M'0 STEP BETA0) as
+      [ALPHA_STEP | (P & STEP_P & MANY_P)].
+    + eapply raw_sn_alpha.
+      * exact M'N_SN.
+      * eapply alpha_equiv_App; [exact ALPHA_STEP | reflexivity].
+    + eapply IHM.
+      * exact BETA0.
+      * econs. exact N_SN.
+      * exact STEP_P.
+      * eapply rawBetaMany_preserves_raw_sn.
+        { eapply rawBetaMany_app_l. exact MANY_P. }
+        { exact M'N_SN. }
+  - eapply IHN.
+    + exact BETA0.
+    + exact STEP.
+    + eapply raw_sn_inv.
+      * exact M'N_SN.
+      * econs 3. exact BETA0.
+Qed.
+
+Lemma rawHead_backward M M'
+  (STEP : rawHeadStep M M')
+  (M'_SN : raw_sn M')
+  : raw_sn M.
+Proof.
+  induction STEP.
+  - eapply raw_wkh_exp_alpha; eassumption.
+  - pose proof (raw_sn_app_inv M' N M'_SN) as (M'_HEAD_SN & N_SN).
+    eapply rawHead_backward_aux.
+    + eapply IHSTEP. exact M'_HEAD_SN.
+    + exact N_SN.
+    + exact STEP.
+    + exact M'_SN.
+Qed.
+
+Fixpoint jmSNe_neutral (M : trm L) (NE : jmSNe M) {struct NE} : neutral M.
+Proof.
+  destruct NE.
+  - econs 1.
+  - econs 2.
+  - econs 3. eapply jmSNe_neutral. exact NE.
+Defined.
+
+Fixpoint jmSN_raw_sn (M : trm L) (M_SN : jmSN M) {struct M_SN} : raw_sn M
+with jmSNe_raw_sn (M : trm L) (M_NE : jmSNe M) {struct M_NE} : raw_sn M
+with jmStep_rawHead (M : trm L) (N : trm L) (STEP : jmStep M N) {struct STEP} : rawHeadStep M N.
+Proof.
+  - destruct M_SN.
+    + eapply jmSNe_raw_sn. exact NE.
+    + eapply raw_sn_lam. eapply jmSN_raw_sn. exact M_SN.
+    + eapply rawHead_backward.
+      * eapply jmStep_rawHead. exact STEP.
+      * eapply jmSN_raw_sn. exact M_SN.
+  - destruct M_NE.
+    + eapply raw_sn_var.
+    + eapply raw_sn_con.
+    + eapply raw_sn_app_neutral.
+      * eapply jmSNe_neutral. exact M_NE.
+      * eapply jmSNe_raw_sn. exact M_NE.
+      * eapply jmSN_raw_sn. exact N_SN.
+  - destruct STEP.
+    + econs 1.
+      * eapply jmSN_raw_sn. exact N_SN.
+      * symmetry. exact ALPHA.
+    + econs 2. eapply jmStep_rawHead. exact STEP.
+Defined.
+
+Fixpoint raw_sn_to_sn_alpha (M : trm L) (M_SN : raw_sn M) {struct M_SN}
+  : forall N, M ≡ₐ N -> sn N.
+Proof.
+  destruct M_SN as [M_SN]. intros N ALPHA. econs. intros P BETA.
+  pose proof (fullBetaOnce_rawBetaOnce N P BETA) as (R & STEP_R & ALPHA_R).
+  pose proof (alpha_rawBetaOnce_comm M N R ALPHA STEP_R) as (Q & STEP_Q & ALPHA_Q).
+  eapply raw_sn_to_sn_alpha.
+  - eapply M_SN. exact STEP_Q.
+  - transitivity R; eassumption.
+Defined.
+
+Definition raw_sn_to_sn (M : trm L) (M_SN : raw_sn M) : sn M :=
+  raw_sn_to_sn_alpha M M_SN M eq_refl.
+
+Theorem Typing_implies_StrongNormalisation {Gamma} {e} {ty}
+  (TYPING : Gamma ⊢ e ⦂ ty)
+  : sn e.
+Proof.
+  pose proof (Typing_implies_jmRed Gamma e ty TYPING nil_subst (jmRedSubst_nil Gamma)) as e_RED.
+  pose proof (jmRed_jmSN ty _ e_RED) as e_JMSN.
+  eapply raw_sn_to_sn_alpha.
+  - eapply jmSN_raw_sn. exact e_JMSN.
+  - symmetry. eapply alpha_equiv_nil_subst.
+Qed.
+
+End STLC_SN.
 
 End STLC_META.
 
